proved contracts for jumps, wip move

src/verification/Contracts.v
@@ -67,24 +67,181 @@ Module Import MSP430Specification <: Specification MSP430Base MSP430Signature MS
                     ; term_var segb1
                     ; term_var segb2 ])).
 
-    Local Notation asn_mpu_pwd_correct mpuctl0 := (asn.formula (formula_user mpu_pwd_correct_p [term_var mpuctl0])).
-    Local Notation asn_ipe_enabled ipectl := (asn.formula (formula_user ipe_enabled_p [term_var ipectl])).
-    Local Notation asn_ipe_locked ipectl := (asn.formula (formula_user ipe_locked_p [term_var ipectl])).
-    Local Notation asn_ipe_unlocked ipectl := (asn.formula (formula_user ipe_unlocked_p [term_var ipectl])).
+    Local Notation asn_accessible_addresses_without pc ipectl segb1 segb2 addr :=
+      (asn.chunk (chunk_user accessible_addresses_without
+                    [ term_var pc
+                    ; term_var ipectl
+                    ; term_var segb1
+                    ; term_var segb2
+                    ; term_var addr])).
 
-    Local Notation asn_access_allowed ipectl segb1 segb2 am pc addr :=
-      (asn.formula
-         (formula_user access_allowed_p
-            [ term_var ipectl; term_var segb1; term_var segb2
-            ; term_enum Eaccess_mode am; term_var pc; addr])).
+    (* Predicates *)
 
-    Local Notation asn_ipe_entry_point segb1 addr :=
-      (asn.formula (formula_user ipe_entry_point_p [term_var segb1; term_var addr])).
+    Definition asn_mpu_pwd_correct {Σ} (mpuctl0 : Term Σ ty.wordBits) : Assertion Σ :=
+      asn.formula
+        (formula_relop bop.eq
+           (term_vector_subrange 8 8 mpuctl0)
+           (term_val (ty.bvec 8) [bv 0x96])).
 
-    Local Notation asn_in_ipe_segment segb1 segb2 addr :=
-      (asn.formula (formula_user in_ipe_segment_p [term_var segb1; term_var segb2; addr])).
-    Local Notation asn_not_in_ipe_segment segb1 segb2 addr :=
-      (asn.formula (formula_user not_in_ipe_segment_p [term_var segb1; term_var segb2; addr])).
+    Definition asn_ipe_unlocked {Σ} (ipectl : Term Σ ty.wordBits) : Assertion Σ :=
+      asn.formula
+        (formula_relop bop.eq
+           (term_vector_subrange 7 1 ipectl)
+           (term_val (ty.bvec 1) [bv 0x0])).
+
+    Definition word_times_16 {Σ} (w : Term Σ ty.wordBits) : Term Σ ty.int :=
+      (term_binop bop.times
+         (term_unsigned w)
+         (term_val ty.int 16)).
+
+    Definition plus_8 {Σ} (n : Term Σ ty.int) : Term Σ ty.int :=
+      (term_binop bop.plus n (term_val ty.int 8)).
+
+    Definition asn_ipe_entry_point {Σ}
+      (segb1 addr : Term Σ ty.wordBits)
+      : Assertion Σ
+    :=
+      asn.formula
+        (formula_relop bop.eq
+           (plus_8 (word_times_16 segb1))
+           (term_unsigned addr)).
+
+    Definition asn_not_in_ipe_segment {Σ}
+      (segb1 segb2 addr : Term Σ ty.wordBits)
+      : Assertion Σ
+    :=
+      asn.formula (formula_relop bop.lt
+                     (term_unsigned addr)
+                     (word_times_16 segb1))
+      ∨ asn.formula (formula_relop bop.le
+                       (word_times_16 segb2)
+                       (term_unsigned addr)).
+
+    Definition asn_trusted {Σ}
+      (ipectl segb1 segb2 pc : Term Σ ty.wordBits)
+      : Assertion Σ
+    :=
+      asn.formula
+        (formula_or
+
+           (* either IPE disabled... *)
+           (formula_relop bop.eq
+              (term_vector_subrange 6 1 ipectl)
+              (term_val (ty.bvec 1) [bv 0x0]))
+
+           (* ...or PC in IPE segment except first 8 bytes
+              and not an execute read in IVT or RV (9.4.1) (TODO) *)
+           (formula_and
+              (formula_relop bop.le
+                 (plus_8 (word_times_16 segb1))
+                 (term_unsigned pc))
+              (formula_relop bop.lt
+                 (term_unsigned pc)
+                 (word_times_16 segb2)))).
+      (*     (* not execute access in IVT or RV (9.4.1) *) *)
+      (*     /\ ((Z.lt addr 0xFF80 \/ Z.le 0xFFFF addr) *)
+      (*         \/ am <> X)) *)
+
+    Definition asn_untrusted {Σ}
+      (ipectl segb1 segb2 pc : Term Σ ty.wordBits)
+      : Assertion Σ
+    :=
+      asn.formula
+        (formula_and
+
+           (* IPE enabled *)
+           (formula_relop bop.eq
+              (term_vector_subrange 6 1 ipectl)
+              (term_val (ty.bvec 1) [bv 0x1]))
+
+           (* PC outside IPE segment except first 8 bytes
+              or execute read in IVT or RV (9.4.1) (TODO) *)
+           (formula_or
+              (formula_relop bop.lt
+                 (term_unsigned pc)
+                 (plus_8 (word_times_16 segb1)))
+              (formula_relop bop.le
+                 (word_times_16 segb2)
+                 (term_unsigned pc)))).
+      (*     (* not execute access in IVT or RV (9.4.1) *) *)
+      (*     /\ ((Z.lt addr 0xFF80 \/ Z.le 0xFFFF addr) *)
+      (*         \/ am <> X)) *)
+
+    Definition asn_access_allowed {Σ}
+      (ipectl segb1 segb2 : Term Σ ty.wordBits)
+      (am : Term Σ (ty.enum Eaccess_mode))
+      (pc addr : Term Σ ty.wordBits)
+      : Assertion Σ
+    :=
+      asn_not_in_ipe_segment segb1 segb2 addr
+
+      ∨ (am = term_enum Eaccess_mode X
+         ∗ asn_ipe_entry_point segb1 addr)
+
+      ∨ (am = term_enum Eaccess_mode X
+         ∗ asn.formula (formula_relop bop.lt
+                          (term_unsigned pc)
+                          (plus_8 (word_times_16 segb1)))
+         ∗ pc = addr)
+
+      (* XXX ∨ asn_trusted ipectl segb1 segb2 pc *).
+
+    Definition asn_any_registers {Σ} : Assertion Σ :=
+        ∃ "SP"    , SP_reg               ↦ term_var "SP"
+      ∗ ∃ "SRCG1" , SRCG1_reg            ↦ term_var "SRCG1"
+      ∗ ∃ "CG2"   , CG2_reg              ↦ term_var "CG2"
+      ∗ ∃ "R4"    , R4_reg               ↦ term_var "R4"
+      ∗ ∃ "R5"    , R5_reg               ↦ term_var "R5"
+      ∗ ∃ "R6"    , R6_reg               ↦ term_var "R6"
+      ∗ ∃ "R7"    , R7_reg               ↦ term_var "R7"
+      ∗ ∃ "R8"    , R8_reg               ↦ term_var "R8"
+      ∗ ∃ "R9"    , R9_reg               ↦ term_var "R9"
+      ∗ ∃ "R10"   , R10_reg              ↦ term_var "R10"
+      ∗ ∃ "R11"   , R11_reg              ↦ term_var "R11"
+      ∗ ∃ "R12"   , R12_reg              ↦ term_var "R12"
+      ∗ ∃ "R13"   , R13_reg              ↦ term_var "R13"
+      ∗ ∃ "R14"   , R14_reg              ↦ term_var "R14"
+      ∗ ∃ "R15"   , R15_reg              ↦ term_var "R15"
+      ∗ ∃ "LIF"   , LastInstructionFetch ↦ term_var "LIF".
+
+    (* Lemmas *)
+
+    Definition lemma_extract_accessible_ptsto : SepLemma extract_accessible_ptsto :=
+      {| lemma_logic_variables :=
+          [ "addr" :: ty.Address; "m" :: ty.enum Eaccess_mode
+          ; "ipectl" :: ty.wordBits; "segb1" :: ty.wordBits; "segb2" :: ty.wordBits
+          ; "pc" :: ty.wordBits
+          ];
+
+        lemma_patterns := [term_var "addr"; term_var "m"];
+
+        lemma_precondition := ⊤;
+          (*   asn_accessible_addresses "pc" "ipectl" "segb1" "segb2" *)
+          (* ∗ asn_access_allowed *)
+          (*     (term_var "ipectl") (term_var "segb1") (term_var "segb2") *)
+          (*     (term_var "m") (term_var "pc") (term_var "addr"); *)
+
+        lemma_postcondition :=
+          (*   asn_accessible_addresses_without "pc" "ipectl" "segb1" "segb2" "addr" *)
+          (* ∗ *) ∃ "v", asn.chunk (chunk_user ptstomem [term_var "addr"; term_var "v"]);
+      |}.
+
+    Definition lemma_return_accessible_ptsto : SepLemma return_accessible_ptsto :=
+      {| lemma_logic_variables :=
+          [ "addr" :: ty.Address
+          ; "ipectl" :: ty.wordBits; "segb1" :: ty.wordBits; "segb2" :: ty.wordBits
+          ; "pc" :: ty.wordBits
+          ];
+
+        lemma_patterns := [term_var "addr"];
+
+        lemma_precondition :=
+            (* asn_accessible_addresses_without "pc" "ipectl" "segb1" "segb2" "addr" *)
+          (* ∗ *) ∃ "v", asn.chunk (chunk_user ptstomem [term_var "addr"; term_var "v"]);
+
+        lemma_postcondition := ⊤
+          (* asn_accessible_addresses "pc" "ipectl" "segb1" "segb2" *);
+      |}.
 
     (* Foreign function contracts *)
 
@@ -125,16 +282,17 @@ Module Import MSP430Specification <: Specification MSP430Base MSP430Signature MS
 
     (* μSail function contracts *)
 
+    (*
     Definition sep_contract_check_ipe_access :
       SepContractFun check_ipe_access :=
       {|
         sep_contract_logic_variables :=
-          [ "addr"     :: ty.Address
-          ; "m"        :: ty.enum Eaccess_mode
-          ; "ipectl"   :: ty.wordBits
-          ; "segb1" :: ty.wordBits
-          ; "segb2" :: ty.wordBits
-          ; "pc"       :: ty.wordBits          ];
+          [ "addr"   :: ty.Address
+          ; "m"      :: ty.enum Eaccess_mode
+          ; "ipectl" :: ty.wordBits
+          ; "segb1"  :: ty.wordBits
+          ; "segb2"  :: ty.wordBits
+          ; "pc"     :: ty.wordBits          ];
 
         sep_contract_localstore := [term_var "addr"; term_var "m"];
 
@@ -143,12 +301,184 @@ Module Import MSP430Specification <: Specification MSP430Base MSP430Signature MS
           ∗ MPUIPC0_reg    ↦ term_var "ipectl"
           ∗ MPUIPSEGB1_reg ↦ term_var "segb1"
           ∗ MPUIPSEGB2_reg ↦ term_var "segb2"
-          ∗ asn_access_allowed "ipectl" "segb1" "segb2" R "pc" (term_var "addr");
 
         sep_contract_result        := "v";
-        sep_contract_postcondition := ⊤ (* term_var "v" = term_val ty.bool true  XXX *);
+        sep_contract_postcondition :=
+            PC_reg         ↦ term_var "pc"
+          ∗ MPUIPC0_reg    ↦ term_var "ipectl"
+          ∗ MPUIPSEGB1_reg ↦ term_var "segb1"
+          ∗ MPUIPSEGB2_reg ↦ term_var "segb2"
+          ∗ (asn_access_allowed
+              (term_var "ipectl") (term_var "segb1") (term_var "segb2")
+              (term_var "m") (term_var "pc") (term_var "addr")
+             ∗ term_var "v" = term_val ty.bool true
+             ∨ term_var "v" = term_val ty.bool false); (* XXX maybe needs asn_not_access_allowed? *)
+      |}. *)
+
+    Definition sep_contract_check_byte_access :
+      SepContractFun check_byte_access :=
+      {|
+        sep_contract_logic_variables :=
+          [ "addr"   :: ty.Address
+          ; "m"      :: ty.enum Eaccess_mode
+          ; "ipectl" :: ty.wordBits
+          ; "segb1"  :: ty.wordBits
+          ; "segb2"  :: ty.wordBits
+          ; "pc"     :: ty.wordBits          ];
+
+        sep_contract_localstore := [term_var "addr"; term_var "m"];
+
+        sep_contract_precondition :=
+            PC_reg         ↦ term_var "pc"
+          ∗ MPUIPC0_reg    ↦ term_var "ipectl"
+          ∗ MPUIPSEGB1_reg ↦ term_var "segb1"
+          ∗ MPUIPSEGB2_reg ↦ term_var "segb2";
+
+        sep_contract_result        := "v";
+        sep_contract_postcondition :=
+            PC_reg         ↦ term_var "pc"
+          ∗ MPUIPC0_reg    ↦ term_var "ipectl"
+          ∗ MPUIPSEGB1_reg ↦ term_var "segb1"
+          ∗ MPUIPSEGB2_reg ↦ term_var "segb2"
+          ∗ asn_access_allowed
+              (term_var "ipectl") (term_var "segb1") (term_var "segb2")
+              (term_var "m") (term_var "pc") (term_var "addr");
       |}.
 
+    Definition sep_contract_set_pc :
+      SepContractFun setPC :=
+      {|
+        sep_contract_logic_variables :=
+          [ "mpuctl0" :: ty.wordBits; "ipectl" :: ty.wordBits
+          ; "segb1" :: ty.wordBits; "segb2" :: ty.wordBits
+          ; "pc" :: ty.wordBits; "pc_new" :: ty.wordBits ];
+
+        sep_contract_localstore := [term_var "pc_new"];
+
+        sep_contract_precondition :=
+            asn_any_registers
+
+          ∗ PC_reg         ↦ term_var "pc"
+          ∗ MPUCTL0_reg    ↦ term_var "mpuctl0"
+          ∗ MPUIPC0_reg    ↦ term_var "ipectl"
+          ∗ MPUIPSEGB1_reg ↦ term_var "segb1"
+          ∗ MPUIPSEGB2_reg ↦ term_var "segb2"
+
+          ∗ asn_untrusted
+              (term_var "ipectl") (term_var "segb1")
+              (term_var "segb2") (term_var "pc");
+
+        sep_contract_result          := "u";
+        sep_contract_postcondition   :=
+            term_var "u" = term_val ty.unit tt
+          ∗ asn_any_registers
+
+          ∗ MPUCTL0_reg    ↦ term_var "mpuctl0"
+          ∗ MPUIPC0_reg    ↦ term_var "ipectl"
+          ∗ MPUIPSEGB1_reg ↦ term_var "segb1"
+          ∗ MPUIPSEGB2_reg ↦ term_var "segb2"
+
+          ∗ ∃ "pc_new",
+            ( PC_reg ↦ term_var "pc_new"
+
+            ∗ asn_access_allowed
+                (term_var "ipectl") (term_var "segb1") (term_var "segb2")
+                (term_enum Eaccess_mode X) (term_var "pc") (term_var "pc_new"));
+      |}.
+
+    Definition sep_contract_execute_move :
+      SepContractFun execute :=
+      {|
+        sep_contract_logic_variables :=
+          [ "mpuctl0" :: ty.wordBits; "ipectl" :: ty.wordBits
+          ; "segb1" :: ty.wordBits; "segb2" :: ty.wordBits
+          ; "pc" :: ty.wordBits
+          ; "instr" :: ty.union Uast
+          ];
+
+        sep_contract_localstore := [term_var "instr"];
+
+        sep_contract_precondition :=
+            asn_any_registers
+
+          ∗ PC_reg         ↦ term_var "pc"
+          ∗ MPUCTL0_reg    ↦ term_var "mpuctl0"
+          ∗ MPUIPC0_reg    ↦ term_var "ipectl"
+          ∗ MPUIPSEGB1_reg ↦ term_var "segb1"
+          ∗ MPUIPSEGB2_reg ↦ term_var "segb2"
+
+          ∗ asn_accessible_addresses "pc" "ipectl" "segb1" "segb2"
+
+          ∗ asn_untrusted
+              (term_var "ipectl") (term_var "segb1")
+              (term_var "segb2") (term_var "pc")
+
+          ∗ term_var "instr" =
+              term_union Uast Kdoubleop
+                (term_val (unionk_ty Uast Kdoubleop)
+                   (tt, MOV, BYTE_INSTRUCTION, R4, INDEXED_MODE, R5, REGISTER_MODE));
+
+        sep_contract_result          := "u";
+        sep_contract_postcondition   :=
+            term_var "u" = term_val ty.unit tt
+          ∗ asn_any_registers
+
+          ∗ PC_reg         ↦ term_var "pc"
+          ∗ MPUCTL0_reg    ↦ term_var "mpuctl0"
+          ∗ MPUIPC0_reg    ↦ term_var "ipectl"
+          ∗ MPUIPSEGB1_reg ↦ term_var "segb1"
+          ∗ MPUIPSEGB2_reg ↦ term_var "segb2"
+
+          ∗ asn_accessible_addresses "pc" "ipectl" "segb1" "segb2";
+      |}.
+
+    Definition sep_contract_execute_jump :
+      SepContractFun execute :=
+      {|
+        sep_contract_logic_variables :=
+          [ "mpuctl0" :: ty.wordBits; "ipectl" :: ty.wordBits
+          ; "segb1" :: ty.wordBits; "segb2" :: ty.wordBits
+          ; "pc" :: ty.wordBits
+          ; "instr" :: ty.union Uast
+          ; "jump_arg" :: unionk_ty Uast Kjump ];
+
+        sep_contract_localstore := [term_var "instr"];
+
+        sep_contract_precondition :=
+            asn_any_registers
+
+          ∗ PC_reg         ↦ term_var "pc"
+          ∗ MPUCTL0_reg    ↦ term_var "mpuctl0"
+          ∗ MPUIPC0_reg    ↦ term_var "ipectl"
+          ∗ MPUIPSEGB1_reg ↦ term_var "segb1"
+          ∗ MPUIPSEGB2_reg ↦ term_var "segb2"
+
+          ∗ asn_untrusted
+              (term_var "ipectl") (term_var "segb1")
+              (term_var "segb2") (term_var "pc")
+
+          ∗ term_var "instr" = term_union Uast Kjump (term_var "jump_arg");
+
+        sep_contract_result          := "u";
+        sep_contract_postcondition   :=
+            term_var "u" = term_val ty.unit tt
+          ∗ asn_any_registers
+
+          ∗ MPUCTL0_reg    ↦ term_var "mpuctl0"
+          ∗ MPUIPC0_reg    ↦ term_var "ipectl"
+          ∗ MPUIPSEGB1_reg ↦ term_var "segb1"
+          ∗ MPUIPSEGB2_reg ↦ term_var "segb2"
+
+          ∗ ∃ "pc_new",
+            ( PC_reg ↦ term_var "pc_new"
+
+            ∗ asn_access_allowed
+                (term_var "ipectl") (term_var "segb1") (term_var "segb2")
+                (term_enum Eaccess_mode X) (term_var "pc") (term_var "pc_new"));
+      |}.
+
+
+(*
     Definition sep_contract_read_mem_aux :
       SepContractFun read_mem_aux :=
       {|
@@ -182,6 +512,7 @@ Module Import MSP430Specification <: Specification MSP430Base MSP430Signature MS
           (*     (inc "addr" m↦ term_var "vh" *)
           (*      ∗ term_var "w" = term_union Uwordbyte Kword (term_var "vh" ++ term_var "vl")); *)
       |}.
+*)
 
     Definition sep_contract_execute :
       SepContractFun execute :=
@@ -216,8 +547,8 @@ Module Import MSP430Specification <: Specification MSP430Base MSP430Signature MS
 
               (* IPE control registers can change if the password is correct
                  and they are not locked TODO and they are not protected by IPE? *)
-            ∗ (   asn_mpu_pwd_correct "mpuctl0"
-                ∗ asn_ipe_unlocked "ipectl"
+            ∗ (   asn_mpu_pwd_correct (term_var "mpuctl0")
+                ∗ asn_ipe_unlocked (term_var "ipectl")
 
               ∨ (* otherwise they must stay the same *)
                   term_var "ipectl_new" = term_var "ipectl"
@@ -228,13 +559,16 @@ Module Import MSP430Specification <: Specification MSP430Base MSP430Signature MS
             ∗ PC_reg ↦ term_var "pc_new"
 
             ∗ (* jumps to untrusted sections are always allowed *)
-              ( asn_not_in_ipe_segment "segb1" "segb2" (term_var "pc_new")
+              ( asn_not_in_ipe_segment
+                  (term_var "segb1") (term_var "segb2") (term_var "pc_new")
 
                 (* arbitrary jumps into the IPE segment are allowed only from the IPE segment *)
-              ∨ asn_access_allowed "ipectl_new" "segb1_new" "segb2_new" X "pc" (term_var "pc_new")
+              ∨ asn_access_allowed
+                  (term_var "ipectl_new") (term_var "segb1_new") (term_var "segb2_new")
+                  (term_enum Eaccess_mode X) (term_var "pc") (term_var "pc_new")
 
                 (* untrusted code can only jump to the entry point *)
-              ∨ asn_ipe_entry_point "segb1_new" "pc_new"
+              ∨ asn_ipe_entry_point (term_var "segb1_new") (term_var "pc_new")
               )
 
             ∗ asn_accessible_addresses "pc_new" "ipectl" "segb1_new" "segb2_new");
@@ -244,8 +578,11 @@ Module Import MSP430Specification <: Specification MSP430Base MSP430Signature MS
     Definition CEnv : SepContractEnv :=
       fun Δ τ f =>
         match f with
-          | read_mem_aux => Some sep_contract_read_mem_aux
-          | _ => None
+        | check_byte_access => Some sep_contract_check_byte_access
+        | setPC => Some sep_contract_set_pc
+          (* | read_mem_aux => Some sep_contract_read_mem_aux *)
+          (* | execute => Some sep_contract_execute *)
+        | _ => None
         end.
 
     (* And this definition maps foreign functions to their contracts. *)
@@ -261,6 +598,8 @@ Module Import MSP430Specification <: Specification MSP430Base MSP430Signature MS
     Definition LEnv : LemmaEnv :=
       fun Δ l =>
         match l with
+        | extract_accessible_ptsto => lemma_extract_accessible_ptsto
+        | return_accessible_ptsto => lemma_return_accessible_ptsto
         end.
   End ContractDefKit.
 End MSP430Specification.
@@ -268,7 +607,8 @@ End MSP430Specification.
 (*** VERIFICATION ***)
 
 Import MSP430Specification.
-Import Erasure.notations.
+Import SymProp.notations.
+(* Import Erasure.notations. *)
 
 Module MSP430Executor :=
   MakeExecutor MSP430Base MSP430Signature MSP430Program MSP430Specification.
@@ -276,35 +616,49 @@ Module MSP430Executor :=
 Import MSP430Executor.
 Import MSP430Executor.Symbolic.
 
-Ltac symbolic_simpl :=
+Ltac symbolic_simpl_reflect :=
   apply validcontract_reflect_sound;
   compute;
   constructor;
   cbn.
 
-Ltac symbolic_simpl_with_fuel :=
+Ltac symbolic_simpl_fuel :=
   apply validcontract_reflect_fuel_sound;
   compute;
   constructor;
   cbn.
 
-Ltac symbolic_simpl_with_erasure :=
+Ltac symbolic_simpl_erasure :=
   apply validcontract_with_erasure_sound;
   compute;
   constructor;
   cbn.
 
-Lemma valid_contract_check_ipe_access : Symbolic.ValidContractWithFuel 2 sep_contract_check_ipe_access fun_check_ipe_access.
-Proof. symbolic_simpl_with_fuel. Qed.
 
-Lemma valid_contract_read_mem_aux : Symbolic.ValidContract sep_contract_read_mem_aux fun_read_mem_aux.
+Lemma valid_contract_execute_move : Symbolic.ValidContractWithFuel 100 sep_contract_execute_move fun_execute.
 Proof.
-  symbolic_simpl.
-  intros bw v _ ctl w _ _ Haccess.
-  split.
-  - intro.
-    unfold access_allowed_inst.
-    .
+  compute.
 
-Lemma valid_contract_execute : Symbolic.ValidContractReflect sep_contract_execute fun_execute.
-Proof. reflexivity. Qed.
+
+
+Lemma valid_contract_check_byte_access : Symbolic.ValidContractReflect sep_contract_check_byte_access fun_check_byte_access.
+Proof. Admitted.
+
+Lemma valid_contract_execute_set_pc : Symbolic.ValidContract sep_contract_set_pc fun_setPC.
+Proof. symbolic_simpl_reflect. Qed.
+
+Lemma valid_contract_execute_jump : Symbolic.ValidContractWithFuel 100 sep_contract_execute_jump fun_execute.
+Proof.
+  apply validcontract_reflect_fuel_sound.
+  compute.
+  constructor.
+  cbn [SymProp.safe instprop instprop_formula].
+  intros until v20.
+  intros _ Hpc;
+    repeat split;
+    try intros _;
+    try apply Hpc;
+    (destruct Hpc as [Hpc | Hpc];
+     [right | left]; right;
+     rewrite rightid_and_true; apply Hpc).
+Qed.
