src/verification/Sig.v
@@ -23,19 +23,12 @@ Import ListNotations.
 Open Scope string_scope.
 Open Scope Z_scope.
 
-Inductive PurePredicate : Set :=
-| mpu_pwd_correct_p
-| ipe_enabled_p
-| ipe_locked_p
-| ipe_unlocked_p
-| access_allowed_p
-| in_ipe_segment_p
-| not_in_ipe_segment_p
-| ipe_entry_point_p.
+Inductive PurePredicate : Set := .
 
 Inductive Predicate :=
 | ptstomem
-| accessible_addresses.
+| accessible_addresses
+| accessible_addresses_without.
 
 Section TransparentObligations.
   Local Set Transparent Obligations.
@@ -51,84 +44,17 @@ Module Export MSP430Signature <: Signature MSP430Base.
   Import MSP430Base.
 
   Section PredicateKit.
-    Local Definition get_bit {n} (v : bv n) (i : nat) {p : IsTrue (Nat.leb (i + 1) n)}: bool :=
-      bv.msb (@bv.vector_subrange n i 1 p v).
-
-    (*
-    Definition mpu_pwd_correct_inst (ctl : Val (ty.record Ripe_ctl)) := mpu_pwd_correct ctl = true.
-    Definition mpu_pwd_incorrect_inst (ctl : Val (ty.record Ripe_ctl)) := mpu_pwd_correct ctl = false.
-    Definition ipe_enabled_inst (ctl : Val (ty.record Ripe_ctl)) := ipe_enabled ctl = true.
-    Definition ipe_locked_inst (ctl : Val (ty.record Ripe_ctl)) := ipe_locked ctl = true.
-    Definition ipe_unlocked_inst (ctl : Val (ty.record Ripe_ctl)) := ipe_locked ctl = false.
-    *)
-
-    Definition mpu_pwd_correct_inst (mpuctl0 : Val ty.wordBits) : Prop :=
-      bv.eqb (bv.vector_subrange 8 8 mpuctl0) (bv.of_Z 0x96) = true.
-
-    Definition ipe_enabled_inst (ipectl : Val ty.wordBits) : Prop :=
-      bv.eqb (bv.vector_subrange 6 1 ipectl) (bv.of_Z 1) = true.
-
-    Definition ipe_locked_inst (ipectl : Val ty.wordBits) :=
-      bv.eqb (bv.vector_subrange 7 1 ipectl) (bv.of_Z 1) = true.
-
-    Definition ipe_unlocked_inst (ipectl : Val ty.wordBits) :=
-      bv.eqb (bv.vector_subrange 7 1 ipectl) (bv.of_Z 1) = true.
-
-    Definition access_allowed_inst
-      (ipectl   : Val ty.wordBits)
-      (ipesegb1 : Val ty.wordBits)
-      (ipesegb2 : Val ty.wordBits)
-      (am       : Val (ty.enum Eaccess_mode))
-      (pc       : Val ty.wordBits)
-      (addr     : Val ty.Address)
-      : Prop
-    :=
-      let addr := bv.unsigned addr in
-      let pc   := bv.unsigned pc in
-      let low  := bv.unsigned ipesegb1 * 16 in
-      let high := bv.unsigned ipesegb2 * 16 in
-
-      (* IPE disabled *)
-      ipe_enabled_inst ipectl
-      (* address not in IPE segment *)
-      \/ (Z.lt addr low \/ Z.le high addr)
-      \/ ((* PC in IPE segment except first 8 bytes *)
-          Z.le (low + 8) pc /\ Z.lt pc high
-          (* not execute access in IVT or RV (9.4.1) *)
-          /\ ((Z.lt addr 0xFF80 \/ Z.le 0xFFFF addr)
-              \/ am <> X)).
-
-    Definition in_ipe_segment_inst (segb1 segb2 addr : Val ty.wordBits) :=
-      bv.unsigned segb1 * 16 <= bv.unsigned addr /\ bv.unsigned addr < bv.unsigned segb2 * 16.
-
-    Definition not_in_ipe_segment_inst (segb1 segb2 addr : Val ty.wordBits) :=
-      bv.unsigned segb1 * 16 > bv.unsigned addr \/ bv.unsigned addr >= bv.unsigned segb2 * 16.
-
-    Definition ipe_entry_point_inst (segb1 addr : Val ty.wordBits) :=
-      bv.unsigned segb1 * 16 + 8 = bv.unsigned addr.
 
     Definition 𝑷 := PurePredicate.
 
     (* Maps each pure predicate to a list of arguments with their types. *)
     Definition 𝑷_Ty (p : 𝑷) : Ctx Ty :=
       match p with
-      | mpu_pwd_correct_p | ipe_enabled_p | ipe_locked_p | ipe_unlocked_p => [ty.wordBits]
-      | in_ipe_segment_p | not_in_ipe_segment_p => [ty.wordBits; ty.wordBits; ty.Address]
-      | ipe_entry_point_p => [ty.wordBits; ty.Address]
-      | access_allowed_p => [ty.wordBits; ty.wordBits; ty.wordBits; ty.enum Eaccess_mode; ty.wordBits; ty.Address]
       end.
 
     (* Interprets a pure predicate name as a Coq proposition. *)
     Definition 𝑷_inst (p : 𝑷) : env.abstract Val (𝑷_Ty p) Prop :=
       match p with
-      | mpu_pwd_correct_p    => mpu_pwd_correct_inst
-      | ipe_enabled_p        => ipe_enabled_inst
-      | ipe_locked_p         => ipe_locked_inst
-      | ipe_unlocked_p       => ipe_unlocked_inst
-      | access_allowed_p     => access_allowed_inst
-      | in_ipe_segment_p     => in_ipe_segment_inst
-      | not_in_ipe_segment_p => not_in_ipe_segment_inst
-      | ipe_entry_point_p    => ipe_entry_point_inst
       end.
 
     Instance 𝑷_eq_dec : EqDec 𝑷 := PurePredicate_eqdec.
@@ -140,6 +66,7 @@ Module Export MSP430Signature <: Signature MSP430Base.
       match p with
       | ptstomem => [ty.Address; ty.byteBits]
       | accessible_addresses => [ty.wordBits; ty.wordBits; ty.wordBits; ty.wordBits]
+      | accessible_addresses_without => [ty.wordBits; ty.wordBits; ty.wordBits; ty.wordBits; ty.Address]
       end.
 
     (* 𝑯_is_dup specifies which predicates are duplicable. A spatial predicate can
@@ -160,6 +87,7 @@ Module Export MSP430Signature <: Signature MSP430Base.
       match p with
       | ptstomem => Some (MkPrecise [ty.Address] [ty.byteBits] eq_refl)
       | accessible_addresses => Some (MkPrecise [ty.wordBits; ty.wordBits; ty.wordBits; ty.wordBits] ε eq_refl)
+      | accessible_addresses_without => Some (MkPrecise [ty.wordBits; ty.wordBits; ty.wordBits; ty.wordBits; ty.Address] ε eq_refl)
       end.
 
   End PredicateKit.
